\section{Commutator properties}
\subsection{Power}
\begin{lemma}\label{CommProp}
If the commutator $[T, H]$ commutes with $T$ i.e.
$$[T, H]T~=~T[T, H]\,,$$ then the following holds:
\begin{equation}\label{eq:tkh}
[T^k, H] = kT^{k-1}[T, H]\,.
\end{equation}
\end{lemma}
This is particularly true when $[T, H]$ is a \emph{number} as in \eqref{THcommutator} where
$T$ and $H$ are the time and energy operator respectively.
\begin{proof}
First of all, the \eqref{eq:tkh} is trivially valid for $k = 1$.

For an arbitrary positive integer $k$ there has:
\begin{dmath}\label{tkhrecur}
[T^k, H] = T^{k-1}TH - HT^{k-1}T = T^{k-1}TH - T^{k-1}HT + T^{k-1}HT - HT^{k-1}T \\
    = T^{k-1}[T, H] + [T^{k-1}, H]T
\end{dmath}
Now, iterating the result in \eqref{tkhrecur},
\begin{dmath}\label{tkhrecurplus}
[T^k, H] = T^{k-1}[T, H] + [T^{k-1}, H]T
= T^{k-1}[T, H] + (T^{k-2}[T, H] + [T^{k-2}, H]T)T
= T^{k-1}[T, H] +  T^{k-1}[T, H] + [T^{k-2}, H]T^2
= 2T^{k-1}[T, H] + [T^{k-2}, H]T^2
= \hdots
= nT^{k-1}[T, H] + [T^{k-n}, H]T^n = \hdots
\end{dmath}
where the commutativity hypothesis $[T, H]T = T[T, H]$ has been used to obtain $T^{k-2}[T, H]T = T^{k-1}[T, H]$.

Now, \eqref{tkhrecurplus} can be continued until it reaches $n=k$ when the term
$[T^{k-n}, H]T^n$ vanishes and a result of $kT^{k-1}[T, H]$ follows.
\end{proof}
